Veir/Dialects/LLZK/Cast/OpInfo.lean
@@ -3,6 +3,7 @@ module
 public import Veir.IR.Simp
 public import Veir.IR.OpInfo
 public import Veir.Verifier.Basic
+public import Veir.Dialects.LLZK.Cast.Properties
 meta import Veir.Meta.OpCode
 
 namespace Veir
@@ -20,15 +21,18 @@ deriving Inhabited, Repr, Hashable, DecidableEq
 end LLZK
 
 @[expose, properties_of]
-def LLZK.Cast.propertiesOf (_op : LLZK.Cast) : Type := Unit
+def LLZK.Cast.propertiesOf (_op : LLZK.Cast) : Type := CastProperties
 
 def LLZK.Cast.fromAttrDict
-    (_op : LLZK.Cast) (_attrDict : Std.HashMap ByteArray Attribute) :
-    Except String (LLZK.Cast.propertiesOf _op) := .ok ()
+    (op : LLZK.Cast) (attrDict : Std.HashMap ByteArray Attribute) :
+    Except String (LLZK.Cast.propertiesOf op) :=
+  match op with
+  | .tofelt => CastProperties.fromAttrDict "cast.tofelt" attrDict
+  | .toindex => CastProperties.fromAttrDict "cast.toindex" attrDict
 
 def LLZK.Cast.toAttrDict
-    (_op : LLZK.Cast) (_props : LLZK.Cast.propertiesOf _op) : Std.HashMap ByteArray Attribute :=
-  Std.HashMap.emptyWithCapacity 0
+    (op : LLZK.Cast) (props : LLZK.Cast.propertiesOf op) : Std.HashMap ByteArray Attribute :=
+  props.toAttrDict
 
 def LLZK.Cast.getEffects (_op : LLZK.Cast) (_props : LLZK.Cast.propertiesOf _op) : MemoryEffects :=
   .none
@@ -50,7 +54,22 @@ def LLZK.Cast.verifyLocalInvariants {OpInfo : Type} [IsOpCode OpInfo]
     [HasDialect OpInfo LLZK.Cast] (opType : LLZK.Cast) (op : OperationPtr)
     (ctx : WfIRContext OpInfo) (opIn : op.InBounds ctx.raw) : Except String PUnit := do
   match opType with
-  | .tofelt | .toindex => op.verifyPlainOpCounts ctx opIn 1 1
+  | .tofelt => do
+    op.verifyPlainOpCounts ctx opIn 1 1
+    let operandType := (op.getOperandTypes! ctx.raw)[0]!
+    if !(operandType.val matches Attribute.integerType { bitwidth := 1 } | Attribute.indexType _) then
+      throw "cast.tofelt: Expected operand to have i1 or index type"
+    let resultType := (op.getResultTypes! ctx.raw)[0]!
+    if !(resultType.val matches Attribute.feltType _) then
+      throw "cast.tofelt: Expected result to have FeltType"
+  | .toindex => do
+    op.verifyPlainOpCounts ctx opIn 1 1
+    let operandType := (op.getOperandTypes! ctx.raw)[0]!
+    if !(operandType.val matches Attribute.feltType _) then
+      throw "cast.toindex: Expected operand to have FeltType"
+    let resultType := (op.getResultTypes! ctx.raw)[0]!
+    if !(resultType.val matches Attribute.indexType _) then
+      throw "cast.toindex: Expected result to have index type"
 
 instance : HasOpInfo LLZK.Cast where
   verifyLocalInvariants := LLZK.Cast.verifyLocalInvariants
