Test/LLZK/Bool/invalid.mlir
@@ -1,10 +1,7 @@
 // RUN: not veir-opt %s 2>&1 | filecheck %s
 
-// CHECK: Error verifying input program: bool.assert: Expected 0 result(s)
+// CHECK: Error verifying input program: bool.and: Expected operand 0 to have i1 type
 "builtin.module"() ({
-  "function.def"() <{sym_name = "invalid_bool", function_type = (i1) -> ()}> ({
-^bb0(%a: i1):
-  %0 = "bool.assert"(%a) : (i1) -> i1
-  "function.return"() : () -> ()
-  }) {function.allow_non_native_field_ops} : () -> ()
+^bb0(%a: i32, %b: i32):
+  %0 = "bool.and"(%a, %b) : (i32, i32) -> i1
 }) : () -> ()
