Test/LLZK/Cast/invalid.mlir
@@ -1,7 +1,7 @@
 // RUN: not veir-opt %s 2>&1 | filecheck %s
 
-// CHECK: Error verifying input program: cast.tofelt: Expected 1 operand(s)
+// CHECK: Error verifying input program: cast.tofelt: Expected operand to have i1 or index type
 "builtin.module"() ({
-^bb0():
-  %0 = "cast.tofelt"() : () -> !felt.type
+^bb0(%arg: !felt.type):
+  %0 = "cast.tofelt"(%arg) : (!felt.type) -> !felt.type
 }) : () -> ()
