Test/LLZK/RAM/invalid.mlir
@@ -1,10 +1,7 @@
 // RUN: not veir-opt %s 2>&1 | filecheck %s
 
-// CHECK: Error verifying input program: ram.store: Expected 0 result(s)
+// CHECK: Error verifying input program: ram.store: Expected address operand to have index type
 "builtin.module"() ({
-  "function.def"() <{sym_name = "invalid_ram", function_type = (index, !felt.type) -> ()}> ({
-^bb0(%addr: index, %val: !felt.type):
-  %0 = "ram.store"(%addr, %val) : (index, !felt.type) -> i32
-  "function.return"() : () -> ()
-  }) {function.allow_witness} : () -> ()
+^bb0(%addr: i32, %val: !felt.type):
+  "ram.store"(%addr, %val) : (i32, !felt.type) -> ()
 }) : () -> ()
